Add destructor to LinearBox

framework/LinearBox.h
@@ -4,10 +4,13 @@
 
 namespace LinearBox_s {
 
+  template<typename A>
+  using DestructorFunction = Tuple0 (*)(A);
+
   template <typename A>
-  class SwapLinear {
+  class SwapAffine {
     public:
-      SwapLinear(A a) {
+      SwapAffine(A a) {
         this-> a = a;
       }
 
@@ -23,5 +26,36 @@ namespace LinearBox_s {
     private:
       A a;
   };
+
+  template <typename A>
+  class SwapLinear {
+    public:
+      SwapLinear(A a, DestructorFunction<A> d) {
+        this-> a = a;
+        this-> d = d;
+      }
+
+      A Swap(A a1) {
+        A ret = this->a;
+        this->a = a1;
+        return ret;
+      }
+
+      A Borrow() { 
+        return a;
+      }
+
+      ~SwapLinear() {
+        d(a);
+      }
+    private:
+      A a;
+      DestructorFunction<A> d;
+  };
+
+  template<typename A>
+  DestructorFunction<A> ToDestructor(Tuple0 (*f)(A)) {
+    return f;
+  }
 
 }
