lib/Lang/LinearBox.i.dfy
@@ -1,14 +1,18 @@
 include "LinearBox.s.dfy"
 include "LinearMaybe.s.dfy"
+include "../Base/LinearOption.i.dfy"
 
 module LinearBox {
   import opened LinearBox_s
   import opened LinearMaybe
+  import opened LinearOption
 
+  // Warning: does not automatically deallocate the linear value.
+  // (either Take and deallocate manually, or use BoxedLinearOption, below, to guarantee deallocation)
   class BoxedLinear<A>
   {
-    var data:SwapLinear<maybe<A>>;
-    ghost var Repr:set<object>;
+    var data:SwapAffine<maybe<A>>
+    ghost var Repr:set<object>
 
     predicate Inv()
       reads this, Repr
@@ -35,7 +39,7 @@ module LinearBox {
       ensures !Has()
       ensures fresh(Repr)
     {
-      data := new SwapLinear(empty());
+      data := new SwapAffine(empty());
       Repr := {this, this.data};
     }
 
@@ -45,7 +49,7 @@ module LinearBox {
       ensures Has()
       ensures fresh(Repr)
     {
-      data := new SwapLinear(give(a));
+      data := new SwapAffine(give(a));
       Repr := {this, this.data};
     }
 
@@ -85,4 +89,99 @@ module LinearBox {
     }
   }
 
+  class BoxedLinearOption<A>
+  {
+    var data:SwapLinear<lOption<A>>
+    ghost var Repr:set<object>
+    ghost var DataInv:(lOption<A>)->bool
+
+    predicate Inv()
+      reads this, Repr
+    {
+      && Repr == {this, this.data}
+      && DataInv == data.Inv()
+    }
+
+    function Has():bool
+      requires Inv()
+      reads this, Repr
+    {
+      data.Read().lSome?
+    }
+
+    function Read():A
+      requires Inv()
+      reads this, Repr
+    {
+      var a:A :| true;
+      match data.Read() case lNone => a case lSome(a) => a
+    }
+
+    // TODO: it would be nice if this were DestructorFunction<A>, or just (linear A)->()
+    constructor Empty(d:DestructorFunction<lOption<A>>)
+      requires OfDestructor(d).requires(lNone)
+      ensures Inv()
+      ensures !Has()
+      ensures fresh(Repr)
+      ensures DataInv == OfDestructor(d).requires
+    {
+      data := new SwapLinear(lNone, d);
+      Repr := {this, this.data};
+      DataInv := OfDestructor(d).requires;
+    }
+
+    constructor(linear a:A, d:DestructorFunction<lOption<A>>)
+      requires OfDestructor(d).requires(lSome(a))
+      ensures Inv()
+      ensures Read() == a
+      ensures Has()
+      ensures fresh(Repr)
+      ensures DataInv == OfDestructor(d).requires
+    {
+      data := new SwapLinear(lSome(a), d);
+      Repr := {this, this.data};
+      DataInv := OfDestructor(d).requires;
+    }
+
+    method Take() returns(linear a:A)
+      modifies this, Repr
+      requires Inv()
+      requires Has()
+      requires DataInv(lNone)
+      ensures Inv()
+      ensures !Has()
+      ensures Repr == old(Repr)
+      ensures DataInv == old(DataInv)
+      ensures a == old(Read())
+      ensures DataInv(lSome(a))
+    {
+      linear var x := data.Swap(lNone);
+      linear var lSome(y) := x;
+      a := y;
+    }
+
+    method Give(linear a:A)
+      modifies this, Repr
+      requires Inv()
+      requires !Has()
+      requires DataInv(lSome(a))
+      ensures Inv()
+      ensures Has()
+      ensures a == Read()
+      ensures Repr == old(Repr)
+      ensures DataInv == old(DataInv)
+    {
+      linear var x := data.Swap(lSome(a));
+      linear match x case lNone => {}
+    }
+
+    function method{:caller_must_be_pure} Borrow():(shared a:A)
+      reads this, Repr
+      requires Inv()
+      requires Has()
+      ensures a == Read()
+    {
+      data.Borrow().value
+    }
+  }
 } // module
