lib/Lang/LinearBox.s.dfy
@@ -5,12 +5,13 @@ module {:extern "LinearBox_s"} LinearBox_s {
   // Prevents linear value from being duplicated (because heap objects can't be duplicated,
   // only references to heap objects can be duplicated).
   // Warning: does not necessarily ensure that linear value is deallocated properly.
-  class {:extern} SwapLinear<A>
+  // (use SwapLinear, below, to guarantee deallocation)
+  class {:extern} SwapAffine<A>
   {
     function {:axiom} Read():A
       reads this
 
-    constructor {:extern "LinearBox_s", "SwapLinear"} (linear a:A)
+    constructor {:extern "LinearBox_s", "SwapAffine"} (linear a:A)
       ensures Read() == a
 
     method {:extern} Swap(linear a1:A) returns(linear a2:A)
@@ -23,4 +24,49 @@ module {:extern "LinearBox_s"} LinearBox_s {
       ensures a == Read()
   }
 
+  // Same as SwapAffine, but with a destructor
+  class {:extern} SwapLinear<A>
+  {
+    function {:axiom} Inv():(A)->bool
+      reads this
+
+    function {:axiom} Read():(a:A)
+      reads this
+      ensures Inv()(a)
+
+    constructor {:extern "LinearBox_s", "SwapLinear"} (linear a:A, d:DestructorFunction<A>)
+      requires OfDestructor(d).requires(a)
+      ensures Inv() == OfDestructor(d).requires
+      ensures Read() == a
+
+    method {:extern} Swap(linear a1:A) returns(linear a2:A)
+      requires Inv()(a1)
+      modifies this
+      ensures Inv() == old(Inv())
+      ensures a2 == old(Read())
+      ensures Read() == a1
+
+    function method{:caller_must_be_pure}{:extern} Borrow():(shared a:A)
+      reads this
+      ensures a == Read()
+  }
+
+  type {:extern} DestructorFunction<A>
+
+  function {:axiom} OfDestructor<A>(d:DestructorFunction<A>) : (linear A)-->()
+
+  function method {:extern} ToDestructor<A>(f:(linear A)-->()) : (d:DestructorFunction<A>)
+    ensures OfDestructor(d) == f
+
 } // module
+
+module Test_LinearBox_s {
+  import opened LinearBox_s
+  linear datatype q = Q(b:bool)
+  function method D(linear x:q):() {linear var Q(_) := x; ()}
+  function method D2(shared x:q):() {()}
+  method M()
+  {
+    var s := new SwapLinear<q>(Q(true), ToDestructor<q>(D));
+  }
+}
