lib/Buckets/BucketImpl.i.dfy
@@ -153,15 +153,6 @@ module BucketImpl {
       WeightBucketIs(pkv);
     }
 
-    method Destructor()
-      requires Inv()
-      modifies Repr
-    {
-      if tree != null {
-        KMB.Free(tree);
-      }
-    }
-
     lemma WeightKeySeqIs(psa: PackedKV.PSA.Psa, k: int)
       requires PSA.WF(psa)
       requires 0 <= k <= |psa.offsets|
